program added

MLoadMStore.thy
@@ -5,7 +5,6 @@ begin
 type_synonym val    = nat
 type_synonym memory = "val list"
 
-
 definition empty_memory :: memory where
   "empty_memory = []"
 
@@ -21,8 +20,6 @@ definition mload :: "memory => nat => val option" where
       then Some (mem ! addr)
       else None)"
 
-
-
 (* Tests *)
 
 value "empty_memory"
@@ -36,9 +33,6 @@ value "mstore empty_memory 4 255"
 
 value "mload (mstore empty_memory 4 255) 4"
   (* = Some 255 *)
-(*
-  mload XXX ....
-*)
 
 lemma test_mload_empty:
   "mload empty_memory 0 = None"
@@ -49,7 +43,6 @@ lemma test_mstore_basic:
   unfolding mload_def mstore_def empty_memory_def
   by (simp add: nth_append)
 
-
 lemma test_mstore_other_addr_untouched:
   "mload (mstore empty_memory 5 99) 6 = None"
   by (simp add: mload_def mstore_def empty_memory_def)
@@ -58,7 +51,6 @@ lemma test_mstore_multiple:
   "mload (mstore (mstore empty_memory 3 100) 4 200) 4 = Some 200"
   unfolding mload_def mstore_def empty_memory_def
   by (simp add: nth_append nth_list_update)
-
 
 lemma test_mstore_overwrite:
   "mload (mstore (mstore empty_memory 1 11) 1 22) 1 = Some 22"
@@ -74,14 +66,92 @@ lemma test_mstore_and_empty_check:
   unfolding mload_def mstore_def empty_memory_def
   by (simp add: nth_append)
 
-
 lemma test_mstore_zero_addr:
   "mload (mstore empty_memory 0 1) 0 = Some 1"
   by (simp add: mload_def mstore_def empty_memory_def)
 
-section \<open>mcopy  Lemmas\<close>
+section \<open>mcopy \<close>
+
+fun mcopy :: "nat => nat => nat => memory => memory" where
+  "mcopy t f 0 mem = mem"
+| "mcopy t f (Suc s) mem =
+     mcopy (t + 1) (f + 1) s
+       (mstore mem t (case mload mem f of None => 0 | Some v => v))"
+
+value "mcopy 3 0 3 (mstore (mstore (mstore empty_memory 0 1) 1 2) 2 3)"
+(* expected result: [1,2,3,1,2,3] *)
 
 
+(* Let's start with simple unit tests for mcopy *)
+lemma mcopy_single_step:
+  "mcopy 0 0 1 [42] = [42]"
+  by (simp add: mload_def mstore_def)
+
+lemma mcopy_single_step_empty:
+  "mcopy 0 0 1 [] = [0]"
+  by (simp add: mload_def mstore_def)
+
+(* Let's try a simpler two-step case first *)
+lemma mcopy_simple_copy:
+  "mcopy 1 0 1 [5] = [5, 5]"
+  by (simp add: mload_def mstore_def)
+
+lemma mcopy_two_steps:
+  "mcopy 2 0 2 [1, 2] = [1, 2, 1, 2]"
+  by eval
+
+
+(* Helper lemmas for mstore length *)
+lemma mstore_length_in_bounds:
+  "addr < length mem --> length (mstore mem addr v) = length mem"
+  by (simp add: mstore_def)
+
+lemma mstore_length_extend:
+  "addr >= length mem --> length (mstore mem addr v) = addr + 1"
+  by (simp add: mstore_def)
+
+(* Just to verify mcopy actually copies correctly *)
+
+lemma mcopy_correctness_simple:
+  "mload (mcopy 1 0 1 [42]) 1 = Some 42"
+  by eval
+
+
+
+
+section "A tiny example program that stores v at 0 and copies it to 1"
+
+
+definition simple_program :: "val => memory" where
+  "simple_program v = mcopy 1 0 1 (mstore empty_memory 0 v)"
+
+lemma simple_program_test:
+  "simple_program 42 = [42, 42]"
+  by (simp add: simple_program_def mstore_def
+                mload_def empty_memory_def)
+
+lemma store_copy_load_same:
+  "mload (simple_program v) 0 = mload (simple_program v) 1"
+  by (simp add: simple_program_def mstore_def
+                mload_def empty_memory_def)
+
+lemma concrete_store_copy_same:
+  "mload (simple_program 99) 0 = Some 99 \<and>
+   mload (simple_program 99) 1 = Some 99"
+  by (simp add: simple_program_def mstore_def
+                mload_def empty_memory_def)
+
+value "simple_program 0"
+(* = [0, 0] *)
+
+value "simple_program 5"
+(* = [5, 5] *)
+
+value "simple_program 42"
+(* = [42, 42] *)
+
+value "simple_program 99"
+(* = [99, 99] *)
 
 
 end
